concurrency/Modular/verif_template.v
@@ -1,0 +1,72 @@
+Require Import VST.concurrency.conclib.
+Require Import VST.floyd.proofauto.
+Require Import VST.atomics.general_locks.
+Require Import bst.give_up_template.
+Require Import bst.puretree.
+Require Import bst.dataStruct.
+Require Import bst.template.
+Require Import bst.giveup_lib.
+Require Import VST.atomics.verif_lock_atomic.
+Require Import VST.floyd.library.
+
+#[export] Instance CompSpecs : compspecs. make_compspecs prog. Defined.
+Definition Vprog : varspecs.  mk_varspecs prog. Defined.
+
+Definition nodebox_rep (g : gname) (g_root : gname) (sh : share) (lock: val) (nb : val) :=
+  EX (np: val) (lsh : share),
+                data_at sh (tptr (t_struct_node)) np nb *
+                (!!(field_compatible t_struct_node nil np /\ is_pointer_or_null lock) &&
+                field_at lsh t_struct_node [StructField _lock] lock np) *
+                in_tree g g_root np lock.
+
+Definition surely_malloc_spec :=
+  DECLARE _surely_malloc
+   WITH t: type, gv: globals
+   PRE [ size_t ]
+       PROP (and (Z.le 0 (sizeof t)) (Z.lt (sizeof t) Int.max_unsigned);
+                complete_legal_cosu_type t = true;
+                natural_aligned natural_alignment t = true)
+       PARAMS (Vptrofs (Ptrofs.repr (sizeof t))) GLOBALS (gv)
+       SEP (mem_mgr gv)
+    POST [ tptr tvoid ]
+    EX p: _,
+       PROP ()
+       RETURN (p)
+       SEP (mem_mgr gv; malloc_token Ews t p * data_at_ Ews t p).
+
+
+Program Definition insert_spec :=
+  DECLARE _insert
+  ATOMIC TYPE (rmaps.ConstType (val * share * val * Z * val * globals * gname * gname))
+  OBJ M INVS ∅
+  WITH b, sh, lock, x, v, gv, g, g_root
+  PRE [ tptr (tptr t_struct_node), tint, tptr tvoid ]
+    PROP (writable_share sh; and (Z.le Int.min_signed x) (Z.le x Int.max_signed); is_pointer_or_null v)
+    PARAMS (b; Vint (Int.repr x); v) GLOBALS (gv)
+    SEP (mem_mgr gv; nodebox_rep g g_root sh lock b) | (CSS g g_root M)
+  POST[ tvoid ]
+    PROP ()
+    LOCAL ()
+    SEP (mem_mgr gv; nodebox_rep g g_root sh lock b) | (CSS g g_root (<[x:=v]>M)).
+
+(* Definition spawn_spec := DECLARE _spawn spawn_spec. *)
+
+Definition Gprog : funspecs :=
+    ltac:(with_library prog [acquire_spec; release_spec; makelock_spec;
+     surely_malloc_spec;  (* insertOp_spec; traverse_spec; *) insert_spec (*; treebox_new_spec *) ]).
+
+Lemma body_insert: semax_body Vprog Gprog f_insert insert_spec.
+Proof.
+  start_function.
+  unfold nodebox_rep.
+  Intros np.
+  forward_call (t_struct_pn, gv).
+  Intros nb.
+  Intros lsh.
+  forward.
+  forward.
+  sep_apply in_tree_duplicate.
+  set (AS := atomic_shift _ _ _ _ _).
+  set Q1:= fun (b : ( bool * (val * (share * (gname * node_info))))%type) =>
+              if b.1 then AS else AS.
+  (* traverse(pn, x, value) *)
